src/Trace.v
@@ -250,12 +250,12 @@ Inductive trace: AnnoTerm -> Plc ->
                  list Ev -> Prop :=
 | tasp: forall r lr x p,
     trace (aasp r lr x) p [(asp_event (fst r) x p)]
-| tatt: forall r lr x p q tr1 req_loc rpy_loc,
+(*| tatt: forall r lr x p q tr1 req_loc rpy_loc,
     trace x q tr1 ->
     trace (aatt r lr (req_loc,rpy_loc) q x) p
           ((req (fst r) req_loc p q (unanno x) )
              :: tr1 ++
-             [(rpy (pred (snd r)) rpy_loc p q)])
+             [(rpy (pred (snd r)) rpy_loc p q)]) *)
 | tlseq: forall r lr x y p tr0 tr1,
     trace x p tr0 ->
     trace y p tr1 ->
@@ -332,6 +332,7 @@ Proof.
 
       inv H1; try inv H.
       destruct x; constructor; auto. *)
+      (*
     +
       inv_in.
       (*
@@ -367,6 +368,7 @@ Proof.
       inv H; try inv H1.
       rewrite H9; simpl.
       apply evtsattrpy; auto. *)
+*)
     +
       rewrite in_app_iff in *.
       destruct_disjunct.
@@ -427,10 +429,11 @@ Proof.
 *)
   - induction H0; inv H.
     + inv H1; destruct r as [i j]; simpl in *; auto.
+      (*
     + simpl; rewrite in_app_iff; simpl.
       inv H1; auto.
       right; right.
-      repeat find_rewrite; simpl; auto.
+      repeat find_rewrite; simpl; auto. *)
     + rewrite in_app_iff.
       inv H1; auto.
 
@@ -539,6 +542,7 @@ Lemma nodup_trace:
 Proof.
   induction t; intros; inv_wfr; inv H0.
   - constructor; auto; constructor.
+    (*
   - destruct r as [i j]; simpl in *; subst; simpl.
     apply NoDup_cons.
     + intro.
@@ -580,6 +584,7 @@ Proof.
         simpl in *.
         lia.
         solve_by_inversion. *)
+*)
   - apply nodup_append; unfold disjoint_lists; auto; intros; eauto.
 
     (*
@@ -868,6 +873,8 @@ Proof.
 
   (*
   - left. solve_by_inversion. *)
+
+  (*
   -
 
     rewrite in_app_iff in *.
@@ -889,6 +896,7 @@ Proof.
     + inv H5. rewrite in_app_iff.
       right. simpl. left. auto.
      *)
+*)
     
   -
     rewrite in_app_iff; auto.
@@ -1024,6 +1032,13 @@ Ltac inv_prec :=
   | H:prec (?C _) _ _ |- _ => inv H
   end.
 
+Ltac do_evin2 :=
+  match goal with
+  | [H:ev_in _ (?C _),
+       H':ev_in _ (?D _)|- _] =>
+    inv H; inv H'
+  end.
+
 (** The traces associated with an annotated term are compatible with
     its event system. *)
 
@@ -1039,27 +1054,23 @@ Proof.
     try expand_let_pairs;
     inv_prec; simpl; auto. 
 
- (* inv H1; simpl; auto. *)
+  (* inv H1; simpl; auto. *)
+  (*
   -
-    Print do_evin.
-    Ltac do_evin2 :=
-      match goal with
-      | [H:ev_in _ (?C _),
-           H':ev_in _ (?D _)|- _] =>
-         inv H; inv H'
-      end.
 
     do_evin2.
 
     (*
 
     inv H12; inv H11. *)
+    (*
     +
       find_eapply_lem_hyp evsys_tr_in; eauto.
       (*
       eapply evsys_tr_in in H4; eauto. *)
+      
       apply earlier_cons; auto.
-      apply in_app_iff; auto.
+      apply in_app_iff; auto. *)
     +
       do_evin.
       (*
@@ -1067,13 +1078,19 @@ Proof.
       apply earlier_cons; auto.
       apply in_app_iff; auto; right; simpl; auto.
   - solve_by_inversion.
+   *)
+
+  (*
   -
     inv_prec.
     (*
 
     inv H11. *)
+    
     +
       do_evin.
+
+      
       (*
 
       inv H13. *)
@@ -1082,6 +1099,8 @@ Proof.
       eapply evsys_tr_in in H12; eauto. *)
       apply earlier_cons_shift; auto.
       apply earlier_append; auto; simpl; auto.
+     
+    
     +
       find_eapply_hyp_hyp; eauto.
       (*
@@ -1090,6 +1109,7 @@ Proof.
       apply earlier_cons_shift; auto.
       apply earlier_left; auto.
     + solve_by_inversion.
+*)
   -
     find_eapply_lem_hyp evsys_tr_in; eauto.
     find_eapply_lem_hyp evsys_tr_in; eauto.
