src/CVM_Semantics.v
@@ -1,0 +1,110 @@
+Require Import CVM_Instr LTS Term_Defs Term StructTactics Auto.
+
+Require Import List.
+Import ListNotations.
+
+Require Import Coq.Program.Tactics.
+
+Set Nested Proofs Allowed.
+
+Lemma ilseq_decomp: forall r l t1 t2 e e' p tr,
+    well_formed (alseq r l t1 t2) ->
+    CVM_Instr.lstar
+      (iconf (instr_compiler (alseq r l t1 t2)) p e) tr
+      (istop p e') ->
+    exists e' tr' p',
+      CVM_Instr.lstar
+        (iconf (instr_compiler t1) p e) tr'
+        (istop p' e') /\
+      exists tr'',
+        CVM_Instr.lstar
+          (iconf (instr_compiler t2) p' e') tr''
+          (istop p e') /\
+        tr = tr' ++ tr''. 
+
+Proof.
+Admitted.
+
+Lemma instr_pl_immut: forall t p e tr p' e',
+    well_formed t ->
+    CVM_Instr.lstar (iconf (instr_compiler t) p e) tr (istop p' e') ->
+    p = p'.
+Proof.
+Admitted.
+
+Ltac clear_trivs :=
+  repeat 
+  match goal with
+  | [H: ?x = ?x |- _] =>
+    clear H
+  end.
+
+Ltac do_pl_immut :=
+  repeat
+    match goal with
+    | [H: CVM_Instr.lstar (iconf (instr_compiler ?t) ?p _) _ (istop ?p' _),
+          H2: well_formed ?t |- _] =>
+      assert_new_proof_by (p = p')
+                          ltac:(eapply instr_pl_immut; [apply H2 | apply H])  
+    end;
+  subst; clear_trivs.
+
+Ltac inv_lstar :=
+  match goal with
+  | [H: CVM_Instr.lstar (?C _) _ _(*(iconf (?C _) _ _) _ _*) |- _] =>
+    invc H
+  end;
+  try solve_by_inversion.
+
+Ltac inv_istep :=
+  match goal with
+  | [H: Instr_step (iconf (?C _) _ _) _ _ |- _] =>
+    invc H
+  end;
+  try solve_by_inversion.
+
+Lemma cvm_refines_lts_event_ordering_corrolary : forall t ai tr et e e' p (*p' o o'*),
+    well_formed t ->
+    ai = instr_compiler t ->
+    CVM_Instr.lstar (iconf ai p e) tr (istop p e') ->
+    (*copland_compile t (mk_st e [] p o) = (Some tt, (mk_st e' tr p' o')) ->
+    st_trace (run_cvm t
+                     (mk_st e [] p o)) = tr -> *)
+    lstar (conf t p et) tr (stop p (aeval t p et)).
+Proof.
+  intros.
+  generalizeEverythingElse t.
+  induction t; intros.
+  -
+    subst;
+    destruct a;
+      repeat (df; inv_lstar; inv_istep);
+      eapply lstar_tran;
+        try apply stasp;
+        df; inv_lstar.
+  -
+    subst.
+    do_wf_pieces.
+    edestruct ilseq_decomp; eauto.
+    destruct_conjs.
+    subst.
+
+    do_pl_immut.
+
+    econstructor.
+    econstructor.
+    eapply lstar_transitive.
+    eapply lstar_stls.
+
+    eapply IHt1; eauto.
+    
+    eapply lstar_silent_tran.
+    apply stlseqstop.
+    eapply IHt2; eauto.
+Defined.
+
+    
+      
+      
+      
+      
