src/RecordUpdate.v
@@ -1,0 +1,6 @@
+(*
+From here:  https://github.com/tchajed/coq-record-update
+*)
+
+From RecordUpdate Require Export RecordSet.
+Export RecordSetNotations.
