src/Term_system.v
@@ -23,12 +23,12 @@ Set Nested Proofs Allowed.
 Fixpoint ev_sys (t: AnnoTerm) p: EvSys Ev :=
   match t with
   | aasp (i, j) lr x => leaf (i, j) (asp_event i x p)
-  | aatt (i, j) lr (req_loc,rpy_loc) q x =>
+  (*| aatt (i, j) lr (req_loc,rpy_loc) q x =>
     before (i, j)
       (leaf (i, S i) (req i req_loc p q (unanno x)))
       (before (S i, j)
               (ev_sys x q)
-              (leaf (pred j, j) (rpy (pred j) rpy_loc p q)))
+              (leaf (pred j, j) (rpy (pred j) rpy_loc p q))) *)
   | alseq r lr x y => before r (ev_sys x p)
                           (ev_sys y p)
   (*| abseq (i, j) lr s x y =>
@@ -474,6 +474,8 @@ Proof.
   -
 
     inv H0; auto. *)
+
+  (*
   -
 
     repeat inv_sup. auto.
@@ -483,6 +485,8 @@ Proof.
     repeat expand_let_pairs.
     repeat apply before_sup in H3.
     inv H3; auto. *)
+   *)
+  
   -
     find_apply_hyp_hyp'.
     
